src/GPUCSL/Lang.v
@@ -806,9 +806,9 @@ Section NonInter.
   | ty_binop : forall (op : binop) (e1 e2 : exp) (ty1 ty2 : type), 
                 typing_exp e1 ty1 -> typing_exp e2 ty2 ->
                 typing_exp (Ebinop op e1 e2) (join ty1 ty2)
-  | ty_eoff : forall (e1 e2 : exp),
+  | ty_eoff : forall (e1 e2 : exp) ty1 ty2,
       typing_exp e1 ty1 -> typing_exp e2 ty2 ->
-      typing_exp (Ebinop op e1 e2) (join ty1 ty2).
+      typing_exp (Eoff e1 e2) (join ty1 ty2).
 
   Inductive typing_cmd : cmd -> type -> Prop :=
   | ty_skip : forall (pc : type), typing_cmd Cskip pc
